Revise assumptions that describe attacker win.

HML_Strategies_Game.thy
@@ -11,47 +11,41 @@ for
   \<tau> :: \<open>'a\<close> +
 fixes
   strat :: \<open>('s, 'a) c_set_game_node posstrategy\<close> and
-  winning_dist :: \<open>('s, 'a) c_set_game_node \<Rightarrow> nat\<close>
+  attacker_winning_region :: \<open>('s, 'a) c_set_game_node set\<close>
 assumes
-  \<comment>\<open>This assumption seems to create an inconsistency.... :/ Will have to restrict it to non-immediately attacker-won positions (?)\<close>
-  winning_dist_attacker_decreasing:
-    \<open>\<And>pos. player1_position pos \<Longrightarrow> winning_dist (strat pos) < winning_dist pos\<close> and
-  winning_dist_defender_constant:
-    \<open>\<And>pos. player0_position pos \<Longrightarrow> game_move pos pos' \<Longrightarrow>  winning_dist pos' \<le> winning_dist pos\<close>
+  finite_win:
+    \<open>wf {(g, g'). c_set_game_moves g g' \<and>
+      g \<in> attacker_winning_region \<and> g' \<in> attacker_winning_region \<and>
+      (player1_position g \<longrightarrow> g' = strat g)}\<close> and
+  strat_stays_winning:
+    \<open>g \<in> attacker_winning_region \<Longrightarrow> player1_position g \<Longrightarrow>
+      strat g \<in> attacker_winning_region \<and> c_set_game_moves g (strat g)\<close> and
+  defender_keeps_losing:
+    \<open>g \<in> attacker_winning_region \<Longrightarrow> c_set_game_defender_node g \<Longrightarrow> c_set_game_moves g g' \<Longrightarrow>
+      g' \<in> attacker_winning_region\<close>
 begin
-
-lemma INCONSISTENCY:
-  False using winning_dist_attacker_decreasing winning_dist_defender_constant wf_measure[of winning_dist] wf_def
-  oops
 
 text \<open>This construction of attacker formulas from a game only works if \<open>strat\<close> is a (non-cyclic)
   attacker strategy. (If it's winning and sound, the constructed formula should be distinguishing.)\<close>
 
 function attack_formula :: \<open>('s, 'a) c_set_game_node \<Rightarrow> ('a,'s) HML_formula\<close> where
   \<open>attack_formula (AttackerNode p Q) =
-    attack_formula (strat (AttackerNode p Q))\<close>
+    (if (AttackerNode p Q) \<in> attacker_winning_region then attack_formula (strat (AttackerNode p Q)) else HML_true)\<close>
 | \<open>attack_formula (DefenderSimNode a p Q) =
     \<langle>\<tau>\<rangle>\<langle>a\<rangle>(attack_formula (AttackerNode p (dsuccs a Q)))\<close>
 | \<open>attack_formula (DefenderSwapNode p Q) =
     (if Q = {} then HML_true else
-    (HML_weaknor (weak_tau_succs Q) (\<lambda>q. (attack_formula (AttackerNode q {p})))))\<close>
+    (HML_weaknor (weak_tau_succs Q) (\<lambda>q. if q \<in> Q then (attack_formula (AttackerNode q {p})) else HML_true )))\<close>
   using c_set_game_defender_node.cases
   by (auto, blast)
 
 termination attack_formula
-proof -
-  define m where \<open>m \<equiv> \<lambda>pos. if player1_position pos then 2 * winning_dist pos else Suc (2 * winning_dist pos)\<close>
-  thus ?thesis
-    using local.termination[OF wf_measure[of m]]
-      winning_dist_defender_constant winning_dist_attacker_decreasing linorder_not_le
-    unfolding m_def measure_def
-    by (auto simp add: less_Suc_eq_le Suc_double_not_eq_double Suc_lessI)
-qed
-\<comment> \<open>zipperposition thinks that one can still prove an inconsistency here ...? :|\<close>
+  using finite_win strat_stays_winning defender_keeps_losing
+  sorry
 
 thm attack_formula.induct
 
-lemma False using attack_formula.induct sledgehammer
+lemma False using attack_formula.induct oops (*sledgehammer*)
 
 lemma \<open>(\<forall> p Q. P  (strat (AttackerNode p Q)) \<longrightarrow> P (AttackerNode p Q)) \<longrightarrow>
   (\<forall>a p Q. P (AttackerNode p (dsuccs a Q)) \<longrightarrow> P (DefenderSimNode a p Q)) \<longrightarrow> (\<forall>p Q. (\<forall> x. P (AttackerNode x {p})) \<longrightarrow> P (DefenderSwapNode p Q)) \<Longrightarrow> P b\<close>
